Remove 'state' from a crashed program'

Result.v
@@ -5,25 +5,26 @@ Require Import Coq.Classes.RelationClasses.
 Require Import Joinable.
 Require Import Preorder.
 
-Inductive result (A : Type) : Type :=
-  | returnR : A -> result A
-  | crashed : result A
-  | exception : result A.
+Inductive result (A S : Type) : Type :=
+  | returnR : (A*S) -> result A S
+  | crashed : result  A S
+  | exception : S -> result A S.
 
 Section result_preorder.
-Context {A : Type} `{PreorderedSet A}.
+Context {A S: Type} `{PreorderedSet A, PreorderedSet S}.
 
-Inductive result_le : result A -> result A -> Prop :=
-  | result_le_crashed : forall r, result_le r (crashed A)
-  | result_le_exception : result_le (exception A) (exception A)
+Inductive result_le : result A S -> result A S -> Prop :=
+  | result_le_crashed : forall r, result_le r (crashed A S)
+  | result_le_exception : forall s1 s2, 
+      preorder s1 s2 -> result_le (exception A S s1) (exception A S s2)
   | result_le_return : forall a1 a2, 
-      preorder a1 a2 -> result_le (returnR A a1) (returnR A a2).
+      preorder a1 a2 -> result_le (returnR A S a1) (returnR A S a2).
 
 Lemma result_le_refl :
   Reflexive result_le.
 Proof.
   unfold Reflexive. destruct x; constructor.
-  apply preorder_refl.
+  apply preorder_refl. apply preorder_refl.
 Qed.
 
 Lemma result_le_trans :
@@ -32,12 +33,13 @@ Proof.
   unfold Transitive.
   intros x y z H1 H2.
   inversion H1; inversion H2; subst; 
-  try constructor; try inversion H2; subst.
-  injection H6 as H8; subst. eapply preorder_trans.
-  apply H0. apply H5.
+  try constructor; try inversion H2; subst. 
+  injection H7 as H9; subst. eapply preorder_trans.
+  apply H3. apply H6.
+  eapply preorder_trans.  apply H3. apply H8.
 Qed.
 
-Global Instance result_preorder : PreorderedSet (result A) := {
+Global Instance result_preorder : PreorderedSet (result A S) := {
   preorder := result_le;
   preorder_refl := result_le_refl;
   preorder_trans := result_le_trans;
@@ -45,36 +47,38 @@ Global Instance result_preorder : PreorderedSet (result A) := {
 End result_preorder.
 
 Section result_joinable.
-Context {A : Type} `{Joinable A}.
+Context {A S : Type} `{Joinable A, Joinable S}.
 
-Definition join_result (r1 r2 : result A) : result A :=
+Definition join_result (r1 r2 : result A S) : result A S :=
   match r1, r2 with
-  | crashed _, _ | _, crashed _ => crashed A
-  | exception _, exception _ => exception A
-  | returnR _ a1, returnR _ a2 => returnR A (join_op a1 a2)
-  | _ , _ => crashed A
+  | crashed _ _, _ | _, crashed _ _ => crashed A S
+  | exception _ _ s1, exception _ _ s2 => exception A S (join_op s1 s2)
+  | returnR _ _ a1, returnR _ _ a2 => returnR A S (join_op a1 a2)
+  | _ , _ => crashed A S
   end.
 
 Lemma join_result_upperbound_left :
   forall r1 r2, preorder r1 (join_result r1 r2).
 Proof. 
   intros r1 r2. simpl. destruct r1.
-  - destruct r2; simpl; constructor. apply join_upper_bound_left.
+  - destruct r2; simpl; constructor. simpl. apply pair_join_upperbound_left.
   - simpl. constructor.
-  - simpl. destruct r2; simpl; constructor.
+  - simpl. destruct r2; simpl; try constructor.
+    apply join_upper_bound_left.
 Qed.
 
 Lemma join_result_upperbound_right :
   forall r1 r2, preorder r2 (join_result r1 r2).
 Proof. 
   intros r1 r2. simpl. destruct r1.
-  - destruct r2; simpl; constructor.
-    apply join_upper_bound_right.
+  - destruct r2; simpl; constructor. simpl. 
+    apply pair_join_upperbound_right.
   - simpl. constructor.
   - simpl. destruct r2; simpl; constructor.
+    apply join_upper_bound_right.
 Qed.
 
-Global Instance result_joinable : Joinable (result A) := {
+Global Instance result_joinable : Joinable (result A S) := {
   join_op := join_result;
   join_upper_bound_left := join_result_upperbound_left;
   join_upper_bound_right := join_result_upperbound_right;
